Generalizei para mais de três eventos, mas agora vai ficar complexo

DFA.v
@@ -3,53 +3,60 @@ Import ListNotations.
 Require BinIntDef.
 
 Definition state := nat.
-
 Axiom states_num_minus_1 : nat.
-(* Definition states_num_minus_1 := 5. *)
-
 Definition states_num := S states_num_minus_1.
 
-Inductive event := add | rem | oth.
+Inductive event := add | rem | oth (e : nat).
+Axiom other_event_list : list nat.
+Fixpoint nl2el l :=
+  match l with
+    x::l => oth x :: nl2el l |
+     []  => []
+  end.
+Definition event_list := [add; rem] ++ nl2el other_event_list.
 
-(* Definition transition (q:state) e :=
-  match q, e with
-    0, add => 5 |
-    0, rem => 1 |
-    1, add => 2 |
-    2, rem => 3 |
-    3, add => 4 |
-    4, rem => 1 |
-    5, add => 1 |
-    _,  _  => 10
-  end. *)
 Axiom transition : state->event->state.
 
-(* Definition is_marked (q:state) :=
-  match q with
-    _ => false
-  end. *)
 Axiom is_marked : state->bool.
 
 Definition DFA := (states_num, transition, is_marked).
+
+(*
+  The states of the DFA are 0, 1, ... and states_num-1.
+  The initial state is the state 0.
+  The sink state is the state n where n = states_num.
+  The events are the ones in event_list.
+*)
 
 Definition is_sink_state (q:state) := q >= states_num.
 
 Definition is_sink_stateb (q:state) := states_num <=? q.
 
-(*
-  The states of the DFA are {0, 1, ..., states_num-1}.
-  The initial state is the state 0.
-  A sink state is any state n where n >= states_num.
-*)
+Definition event_eq e1 e2 :=
+  match e1, e2 with
+     add  ,  add   => true     |
+     rem  ,  rem   => true     |
+    oth e1, oth e2 => e1 =? e2 |
+      _   ,    _   => false
+  end.
+
+Fixpoint search_event (l:list event) (e:event) :=
+  match l with
+    e'::l => if event_eq e e' then true else search_event l e |
+      _   => false
+  end.
+
+Fixpoint event_is_valid e := search_event event_list e.
 
 Fixpoint xtransition q w :=
-  match w with
-    a::w => if is_sink_stateb q then
-              q
-            else
-              xtransition (transition q a) w |
-    []  => q
-  end.
+  if is_sink_stateb q then states_num else
+    match w with
+      e::w => if event_is_valid e then
+                xtransition (transition q e) w
+              else
+                states_num |
+      []  => q
+    end.
 
 Definition ixtransition w := xtransition 0 w.
 
@@ -59,7 +66,7 @@ Proof.
   reflexivity.
 Qed.
 
-Definition is_proper_transition q e := ~ is_sink_state (xtransition q [e]).
+Definition transition_is_proper q e := ~ is_sink_state (xtransition q [e]).
 
 Definition is_generated w := ~ is_sink_state (ixtransition w).
 
@@ -89,12 +96,19 @@ Proof.
     apply H.
 Qed.
 
+Lemma first_sink_state : is_sink_stateb states_num = true.
+Proof.
+  apply is_sink_stateb__is_sink_state.
+  unfold is_sink_state.
+  omega.
+Qed.
+
 Lemma xtransition_sink_state : forall w q,
-  is_sink_stateb q = true -> xtransition q w = q.
+  is_sink_stateb q = true -> xtransition q w = states_num.
 Proof.
   intros w q H.
   destruct w.
-  - reflexivity.
+  - simpl. rewrite H. reflexivity.
   - simpl.
     rewrite H.
     reflexivity.
@@ -104,14 +118,22 @@ Theorem xtransition_distr : forall w w' q,
   xtransition q (w ++ w') = xtransition (xtransition q w) w'.
 Proof.
   intros w w'.
-  induction w as [|e w IHw].
-  - reflexivity.
-  - intro q.
-    simpl.
-    destruct (is_sink_stateb q) eqn:H0.
-    + symmetry; apply xtransition_sink_state.
-      apply H0.
-    + apply IHw.
+  induction w; intro q.
+  - simpl. destruct (is_sink_stateb q) eqn:eq.
+    + pose proof first_sink_state as H.
+      apply xtransition_sink_state with (w:=w') in H.
+      apply xtransition_sink_state with (w:=w') in eq.
+      rewrite eq, H.
+      reflexivity.
+    + reflexivity.
+  - simpl.
+    pose proof first_sink_state as H.
+    apply xtransition_sink_state with (w:=w') in H.
+    destruct (is_sink_stateb q) eqn:eq.
+    + rewrite H. reflexivity.
+    + destruct (event_is_valid a).
+      * apply IHw.
+      * rewrite H. reflexivity.
 Qed.
 
 Theorem ixtransition_distr : forall w w',
@@ -130,10 +152,5 @@ Proof.
   rewrite xtransition_distr in H.
   apply is_sink_stateb__is_sink_state in H0.
   apply H, is_sink_stateb__is_sink_state.
-  destruct w'.
-  - simpl.
-    apply H0.
-  - simpl.
-    rewrite H0.
-    apply H0.
+  destruct w'; simpl; rewrite H0; apply first_sink_state.
 Qed.
